Algoritmos Aproximados/VertexCover.dfy/VertexCover2Aproximated.dfy
@@ -17,11 +17,8 @@ include "VertexCoverKAproximated.dfy"
 
     Lemmas:
         These lemmas are used to prove that the invariants hold through each iteration of the loop in vertexCover2Aproximated
-        -invariantsHold: Encapsulates all the following invariants
-        -partialSolutionCoversAnalyzedNodes: All edges that we no longer consider are already covered by the partial solution
-        -noIncidentEdgesRemain: All edges that contain a node that belongs to the partial solution have already been analyzed
+        -partialSolutionCoversAnalyzedEdges: All edges that we no longer consider are already covered by the partial solution
         -sizeOfPartialSolution: The size of the partial solution is exactly twice the size of pickedEdges
-        -pickedEdgesAreSubsetOfPartialSolution: For all edges in pickedEdges, both of the nodes it connects belong to the partial solution
         -invariantPickedEdgesHolds: All edges in pickedEdges are disjoint
 
         This lemma proves that the solution obtained after iterating is a 2-Aproximation
@@ -47,58 +44,10 @@ include "VertexCoverKAproximated.dfy"
             optimalVertexCoverExists
 */
 
-//Encapsulates the properties to be maintained while iterating in vertexCover2Aproximated
-predicate invariantLoop(graph: Graph, I: set<Node>, edgesRemaining: set<Edge>, pickedEdges: set<Edge>){
-    isValidGraph(graph) && 
-    I <= graph.0 && 
-    edgesRemaining <= graph.1 &&
-    pickedEdges <= graph.1 &&
-    edgesRemaining * pickedEdges == {} &&
-    (forall e: Edge | e in edgesRemaining :: e * I == {}) &&
-    (forall e: Edge | e in graph.1 - edgesRemaining :: |I * e| > 0) &&
-    (forall v: Node, e: Edge | v in graph.0 && e in graph.1 && v in I && v in e :: e !in edgesRemaining) &&
-    |I| == |pickedEdges| * 2 &&
-    (forall e: Edge|  e in graph.1 && e in pickedEdges :: e <= I) &&
-    (forall e1, e2 | e1 in pickedEdges && e2 in pickedEdges && e1 != e2 :: e1 * e2 == {})
-}
-
-//The invariants of the loop in vertexCover2Aproximated hold 
-//Used locally by bodyLoop
-//For all invariants whose proof is not trivial, we call a lemma that proves that invariant holds
-lemma invariantsHold(graph: Graph, edgesRemaining: set<Edge>, pickedEdges: set<Edge>, e: Edge, I: set<Node>, 
-                     edgesRemaining': set<Edge>, pickedEdges': set<Edge>, I': set<Node>)
-requires invariantLoop(graph, I, edgesRemaining, pickedEdges)
-requires edgesRemaining != {} 
-requires e in edgesRemaining
-requires edgesRemaining' == edgesRemaining - incidentEdgesToEdge(graph, e)
-requires pickedEdges' == pickedEdges + {e}
-requires I' == I + e
-ensures invariantLoop(graph, I', edgesRemaining', pickedEdges')
-ensures edgesRemaining' < edgesRemaining
-{
-    //isValidGraph(graph)
-    //I <= graph.0 
-    //edgesRemaining <= graph.1 
-    //pickedEdges <= graph.1 
-    //edgesRemaining * pickedEdges == {} 
-    //forall e: Edge | e in edgesRemaining :: e * I == {} 
-
-    //forall e: Edge | e in graph.1 - edgesRemaining :: |I * e| > 0
-    partialSolutionCoversAnalyzedNodes(graph, edgesRemaining, I, e);
-    //forall v: Node, e: Edge | v in graph.0 && e in graph.1 && v in I && v in e :: e !in edgesRemaining 
-    noIncidentEdgesRemain(graph, I, edgesRemaining);
-    //|I| == |pickedEdges| * 2
-    sizeOfPartialSolution(I, pickedEdges, e);
-    //(forall e: Edge, n1: Node, n2: Node | n1 in graph.0 && n2 in graph.0 &&  n1 < n2 && e in graph.1 && e in pickedEdges && e == {n1, n2} :: n1 in I && n2 in I)
-    pickedEdgesAreSubsetOfPartialSolution(graph, pickedEdges, e, I, pickedEdges', I');
-    //(forall e1, e2 | e1 in pickedEdges && e2 in pickedEdges && e1 != e2 :: e1 * e2 == {})
-    invariantPickedEdgesHolds(graph, edgesRemaining, pickedEdges, e, I, edgesRemaining', pickedEdges', I');
-}
-
 //All edges that we no longer consider are already covered by the partial solution
-//Used locally by invariantsHold
+//Used locally by bodyLoop
 //Proof is trivial if you divide by cases
-lemma partialSolutionCoversAnalyzedNodes(graph: Graph, edgesRemaining: set<Edge>, I: set<Node>, e: Edge)
+lemma partialSolutionCoversAnalyzedEdges(graph: Graph, edgesRemaining: set<Edge>, I: set<Node>, e: Edge)
 requires isValidGraph(graph)
 requires edgesRemaining <= graph.1
 requires e in graph.1
@@ -116,22 +65,9 @@ ensures forall e': Edge | e' in graph.1 - (edgesRemaining - incidentEdgesToEdge(
     }
 }
 
-//All edges that contain a node that belongs to the partial solution have already been analyzed
-//Used locally by invariantsHold
-//Trivial proof
-lemma noIncidentEdgesRemain(graph: Graph, I: set<Node>, edgesRemaining: set<Edge>)
-requires isValidGraph(graph)
-requires I <= graph.0
-requires edgesRemaining <= graph.1
-requires forall e: Edge | e in graph.1 - edgesRemaining :: |I * e| > 0
-requires forall e: Edge | e in edgesRemaining :: e * I == {}
-requires forall v: Node, e: Edge | v in graph.0 && e in graph.1 && v in I && v in e :: e !in edgesRemaining 
-ensures forall v: Node, e: Edge | v in graph.0 && e in graph.1 && v in I + e && v in e :: e !in edgesRemaining - incidentEdgesToEdge(graph, e)
-{ }
-
 //The size of the partial solution is exactly twice the size of pickedEdges
 //because each iteration we add both vertices from the picked edge to the partial solution
-//Used locally by invariantsHold
+//Used locally by bodyLoop
 lemma sizeOfPartialSolution(I: set<Node>, pickedEdges: set<Edge>, e: Edge)
 requires I * e == {}
 requires |e| == 2
@@ -143,34 +79,20 @@ ensures |I + e| == |pickedEdges + {e}| * 2
     cardinalitySum(pickedEdges, {e});
 }
 
-//For all edges in pickedEdges, both of the nodes it connects belong to the partial solution
-//Used by invariantsHold
-//Trivial proof
-lemma pickedEdgesAreSubsetOfPartialSolution(graph: Graph, pickedEdges: set<Edge>, e: Edge, I: set<Node>, pickedEdges': set<Edge>, I': set<Node>)
-requires isValidGraph(graph) 
-requires I <= graph.0 
-requires pickedEdges <= graph.1 
-requires |I| == |pickedEdges| * 2
-requires (forall e: Edge | e in graph.1 && e in pickedEdges :: e <= I)
-requires pickedEdges' == pickedEdges + {e}
-requires I' == I + e
-ensures (forall e: Edge | e in graph.1 && e in pickedEdges' :: e <= I')
-{ }
-
 //All edges in pickedEdges are disjoint
-//Used locally by invariantsHold
+//Used locally by bodyLoop
 //Proof is trivial after dividing into cases
 lemma invariantPickedEdgesHolds(graph: Graph, edgesRemaining: set<Edge>, pickedEdges: set<Edge>, e: Edge, I: set<Node>, 
-                                edgesRemaining': set<Edge>, pickedEdges': set<Edge>, I': set<Node>)
+                                edgesRemainingN: set<Edge>, pickedEdgesn: set<Edge>, In: set<Node>)
 requires invariantLoop(graph, I, edgesRemaining, pickedEdges)
 requires edgesRemaining != {} 
 requires e in edgesRemaining
-requires edgesRemaining' == edgesRemaining - incidentEdgesToEdge(graph, e)
-requires pickedEdges' == pickedEdges + {e}
-requires I' == I + e
-ensures forall e1, e2 | e1 in pickedEdges' && e2 in pickedEdges' && e1 != e2 :: e1 * e2 == {}
+requires edgesRemainingN == edgesRemaining - incidentEdgesToEdge(graph, e)
+requires pickedEdgesn == pickedEdges + {e}
+requires In == I + e
+ensures forall e1, e2 | e1 in pickedEdgesn && e2 in pickedEdgesn && e1 != e2 :: e1 * e2 == {}
 {
-    forall e1, e2 | e1 in pickedEdges' && e2 in pickedEdges' && e1 != e2 
+    forall e1, e2 | e1 in pickedEdgesn && e2 in pickedEdgesn && e1 != e2 
     ensures e1 * e2 == {}
     {
         if (e1 != e && e2 != e) { 
@@ -183,26 +105,6 @@ ensures forall e1, e2 | e1 in pickedEdges' && e2 in pickedEdges' && e1 != e2 :: 
             assert e1 in pickedEdges; 
         }
     }
-}
-
-//Encapsulates the operation to be performed each iteration of the loop in vertexCover2Aproximated
-//This consists of picking an edge that has yet to be covered by the partial solution, 
-//and adding both of the vertices it coneects to the partial solution, then updating the set of covered edges
-//Used locally by vertexCover2Aproximated
-method bodyLoop(graph: Graph, I: set<Node>, edgesRemaining: set<Edge>, pickedEdges: set<Edge>) 
-returns (I': set<Node>, edgesRemaining': set<Edge>, pickedEdges': set<Edge>)
-requires invariantLoop(graph, I, edgesRemaining, pickedEdges)
-requires edgesRemaining != {} 
-ensures invariantLoop(graph, I', edgesRemaining', pickedEdges')
-ensures edgesRemaining' < edgesRemaining
-{
-    var e := pick(edgesRemaining);
-    
-    pickedEdges' := pickedEdges + {e};
-    I' := I + e;  
-    edgesRemaining' := edgesRemaining - incidentEdgesToEdge(graph, e);
-    
-    invariantsHold(graph, edgesRemaining, pickedEdges, e, I, edgesRemaining', pickedEdges', I');
 }
 
 //An optimal solution must cover all edges that were picked during the construction of the aproximated solution
@@ -222,6 +124,44 @@ ensures |O| >= |pickedEdges|
         var n2 :| n2 in e && n2 != n1;
         optimalSolutionCoversPickedEdges(graph, O - {n1, n2}, pickedEdges - {e});
     }
+}
+
+//Encapsulates the properties to be maintained while iterating in vertexCover2Aproximated
+predicate invariantLoop(graph: Graph, I: set<Node>, edgesRemaining: set<Edge>, pickedEdges: set<Edge>){
+    isValidGraph(graph) && 
+    I <= graph.0 && 
+    edgesRemaining <= graph.1 &&
+    pickedEdges <= graph.1 &&
+    (forall e: Edge | e in edgesRemaining :: e * I == {}) &&
+    (forall e: Edge | e in graph.1 - edgesRemaining :: |I * e| > 0) &&
+    |I| == |pickedEdges| * 2 &&
+    (forall e: Edge|  e in graph.1 && e in pickedEdges :: e <= I) &&
+    (forall e1, e2 | e1 in pickedEdges && e2 in pickedEdges && e1 != e2 :: e1 * e2 == {})
+}
+
+//Encapsulates the operation to be performed each iteration of the loop in vertexCover2Aproximated
+//This consists of picking an edge that has yet to be covered by the partial solution, 
+//and adding both of the vertices it coneects to the partial solution, then updating the set of covered edges
+//Used locally by vertexCover2Aproximated
+method bodyLoop(graph: Graph, I: set<Node>, edgesRemaining: set<Edge>, pickedEdges: set<Edge>) 
+returns (In: set<Node>, edgesRemainingN: set<Edge>, pickedEdgesn: set<Edge>)
+requires invariantLoop(graph, I, edgesRemaining, pickedEdges)
+requires edgesRemaining != {} 
+ensures invariantLoop(graph, In, edgesRemainingN, pickedEdgesn)
+ensures edgesRemainingN < edgesRemaining
+{
+    var e := pick(edgesRemaining);
+    
+    pickedEdgesn := pickedEdges + {e};
+    In := I + e;  
+    edgesRemainingN := edgesRemaining - incidentEdgesToEdge(graph, e);
+    
+    //forall e: Edge | e in graph.1 - edgesRemaining :: |I * e| > 0
+    partialSolutionCoversAnalyzedEdges(graph, edgesRemaining, I, e);
+    //|I| == |pickedEdges| * 2
+    sizeOfPartialSolution(I, pickedEdges, e);
+    //(forall e1, e2 | e1 in pickedEdges && e2 in pickedEdges && e1 != e2 :: e1 * e2 == {})
+    invariantPickedEdgesHolds(graph, edgesRemaining, pickedEdges, e, I, edgesRemainingN, pickedEdgesn, In);
 }
 
 //Method that constructs a 2-Aproximated solution to the Vertex Cover Problem
@@ -266,3 +206,63 @@ ensures isKAproximatedVertex(graph, I, 2)
         }
     }
 }
+
+//////////////////////////////////////////////////
+//               Currently Unused               //
+//////////////////////////////////////////////////
+
+/*
+
+//The invariants of the loop in vertexCover2Aproximated hold 
+//For all invariants whose proof is not trivial, we call a lemma that proves that invariant holds
+lemma invariantsHold(graph: Graph, edgesRemaining: set<Edge>, pickedEdges: set<Edge>, e: Edge, I: set<Node>, 
+                     edgesRemainingN: set<Edge>, pickedEdgesn: set<Edge>, In: set<Node>)
+requires invariantLoop(graph, I, edgesRemaining, pickedEdges)
+requires edgesRemaining != {} 
+requires e in edgesRemaining
+requires edgesRemainingN == edgesRemaining - incidentEdgesToEdge(graph, e)
+requires pickedEdgesn == pickedEdges + {e}
+requires In == I + e
+ensures invariantLoop(graph, In, edgesRemainingN, pickedEdgesn)
+ensures edgesRemainingN < edgesRemaining
+{
+    //isValidGraph(graph)
+    //I <= graph.0 
+    //edgesRemaining <= graph.1 
+    //pickedEdges <= graph.1 
+    //edgesRemaining * pickedEdges == {} 
+    //forall e: Edge | e in edgesRemaining :: e * I == {} 
+
+    //forall e: Edge | e in graph.1 - edgesRemaining :: |I * e| > 0
+    partialSolutionCoversAnalyzedEdges(graph, edgesRemaining, I, e);
+    //|I| == |pickedEdges| * 2
+    sizeOfPartialSolution(I, pickedEdges, e);
+    //(forall e1, e2 | e1 in pickedEdges && e2 in pickedEdges && e1 != e2 :: e1 * e2 == {})
+    invariantPickedEdgesHolds(graph, edgesRemaining, pickedEdges, e, I, edgesRemainingN, pickedEdgesn, In);
+}
+
+//All edges that contain a node that belongs to the partial solution have already been analyzed
+//Trivial proof
+lemma noIncidentEdgesRemain(graph: Graph, I: set<Node>, edgesRemaining: set<Edge>)
+requires isValidGraph(graph)
+requires I <= graph.0
+requires edgesRemaining <= graph.1
+requires forall e: Edge | e in graph.1 - edgesRemaining :: |I * e| > 0
+requires forall e: Edge | e in edgesRemaining :: e * I == {}
+requires forall v: Node, e: Edge | v in graph.0 && e in graph.1 && v in I && v in e :: e !in edgesRemaining 
+ensures forall v: Node, e: Edge | v in graph.0 && e in graph.1 && v in I + e && v in e :: e !in edgesRemaining - incidentEdgesToEdge(graph, e)
+{ }
+
+//For all edges in pickedEdges, both of the nodes it connects belong to the partial solution
+//Trivial proof
+lemma pickedEdgesAreSubsetOfPartialSolution(graph: Graph, pickedEdges: set<Edge>, e: Edge, I: set<Node>, pickedEdgesn: set<Edge>, In: set<Node>)
+requires isValidGraph(graph) 
+requires I <= graph.0 
+requires pickedEdges <= graph.1 
+requires |I| == |pickedEdges| * 2
+requires (forall e: Edge | e in graph.1 && e in pickedEdges :: e <= I)
+requires pickedEdgesn == pickedEdges + {e}
+requires In == I + e
+ensures (forall e: Edge | e in graph.1 && e in pickedEdgesn :: e <= In)
+{ }
+*/
